theories/hoare.v
@@ -3,8 +3,7 @@ Require Import Regex2NFA.theories.st_graph_nfa.
 Require Import Regex2NFA.theories.st_nograph_nfa.
 Require Import Regex2NFA.theories.regex.
 Require Import Coq.ZArith.ZArith.
-From StateMonad.monaderror Require Import monadEbasic.
-From StateMonad.monaderror Require Import monadEhoare.
+From StateMonad.monaderror Require Import monadEbasic monadEwhile monadesafe_lib monadEhoare.
 
 Import MonadNotation.
 Local Open Scope stmonad_scope.
@@ -12,13 +11,34 @@ Local Open Scope Z_scope.
 
 (** high_level prop *)
 Lemma st_nograph_inc {T: Type} :
-  forall (G: @pg_nfa T) (r: reg_exp T), exists (v e : Z),
-  Hoare (fun s1 => s1.(max_v) = v /\
-                   s1.(max_e) = e)
+  forall (r: reg_exp T), exists (v e : Z),
+  Hoare (fun s1 => s1.(max_v) = v /\ s1.(max_e) = e)
         (regexToNFA r)
-        (fun el s2 => el.(startVertex) >= v /\
-                      el.(endVertex) >= v /\
-                      G_disjoint G el.(graph) ).
+        (fun el s2 => let G := el.(graph) in
+                      let g := G.(pg) in
+                      s2.(max_v) > v /\
+                      s2.(max_e) > e /\
+                      (forall n, g.(vvalid) n -> v < n <= s2.(max_v)) /\
+                      (forall n, g.(evalid) n -> e < n <= s2.(max_e)) /\
+                      forall str, exp_match r str <->
+                                  G_match_string G el.(startVertex) el.(endVertex) str
+        ).
+Proof.
+Admitted.
+
+Lemma st_graph_inc {T: Type} :
+  forall (r : reg_exp T), exists (v e : Z) (G: @pg_nfa T),
+  Hoare (fun s1 => s1.(max_v') = v /\
+                   s1.(max_e') = e /\
+                   s1.(st_graph) = G)
+        (regexToNFA' r)
+        (fun el s2 => let g := G.(pg) in
+                      s2.(max_v') > v /\
+                      s2.(max_e') > e /\
+                      (forall n, g.(vvalid) n -> n <= s2.(max_v')) /\
+                      (forall n, g.(evalid) n -> n <= s2.(max_e'))
+                      (** TODO: safeExec *)
+        ).
 Proof.
 Admitted.
 
